implementing #38; explicitly bound type-variables need not begin with a prime ... see millionaires.fst for uses of this new syntax ... starting to migrate prims.fst to the syntax too; of course, the primed variable syntax is still there for compatibility with ML

src/absyn/print.fs
@@ -97,7 +97,7 @@ and typ_to_string x =
   | Typ_delayed _ -> failwith "impossible"
   | Typ_meta(Meta_named(_, l)) -> sli l
   | Typ_meta meta ->           Util.format1 "(Meta %s)" (meta|> meta_to_string)
-  | Typ_btvar btv -> strBvd btv.v 
+  | Typ_btvar btv -> strBvd btv.v
     //Util.format2 "(%s:%s)" (strBvd btv.v) (kind_to_string x.tk)
   | Typ_const v -> sli v.v //Util.format2 "%s:%s" (sli v.v) (kind_to_string x.tk)
   | Typ_fun(binders, c) ->     Util.format2 "(%s -> %s)"  (binders_to_string " -> " binders) (comp_typ_to_string c)
