lib/prims.fst
@@ -24,61 +24,63 @@ logic type l_and : Binop (* infix binary '/\' *)
 logic type l_or  : Binop (* infix binary '\/' *)
 logic type l_iff : Binop (* infix binary '<==>' *)
 logic type l_imp : Binop (* infix binary '==>' *)
-logic type Forall : #'a:Type -> ('a -> Type) -> Type 
-logic type Exists : #'a:Type -> ('a -> Type) -> Type 
+logic type Forall : #a:Type -> (a -> Type) -> Type 
+logic type Exists : #a:Type -> (a -> Type) -> Type 
 logic type ForallTyp : (Type -> Type) -> Type (* Handled specially to support quantification over types of arbitrary kinds *)
 logic type ExistsTyp : (Type -> Type) -> Type (* Handled specially to support quantification over types of arbitrary kinds *)
 logic type True 
 logic type False
 logic type EqTyp : Type -> Type -> Type                    (* infix binary '==' *)
-logic type Eq2 : #'a:Type -> #'b:Type -> 'a -> 'b -> Type  (* infix binary '==' *)
-logic type XOR 'P 'Q = ('P \/ 'Q) /\ ~('P /\ 'Q)
+logic type Eq2 : #a:Type -> #b:Type -> a -> b -> Type  (* infix binary '==' *)
+logic type XOR (p:Type) (q:Type) = (p \/ q) /\ ~(p /\ q)
 logic type ITE : Type -> Type -> Type -> Type (* written if/then/else in concrete syntax *)
-logic type Precedes : #'a:Type -> #'b:Type -> 'a -> 'b -> Type  (* a built-in well-founded partial order over all terms *)
+logic type Precedes : #a:Type -> #b:Type -> a -> b -> Type  (* a built-in well-founded partial order over all terms *)
+assume type bool
+logic type b2t (b:bool) = b==true
 
 monad_lattice { (* The definition of the PURE effect is fixed; no user should ever change this *)
   PURE::
              terminating
              kind Pre = Type
-             kind Post ('a:Type) = 'a -> Type
-             kind WP ('a:Type) = Post 'a -> Pre
-             type return ('a:Type) (x:'a) ('p:Post 'a) = 'p x
-             type bind_wp  ('a:Type) ('b:Type) ('wp1:WP 'a) ('wlp1:WP 'a) 
-                                               ('wp2: 'a -> WP 'b) ('wlp2:'a -> WP 'b) 
-                                               ('p:Post 'b) = 'wp1 (fun a -> 'wp2 a 'p)
-             type bind_wlp ('a:Type) ('b:Type) ('wlp1:WP 'a) 
-                                               ('wlp2:'a -> WP 'b) 
-                                               ('p:Post 'b) = 'wlp1 (fun a -> 'wlp2 a 'p)
-             type if_then_else ('a:Type) ('p:Type) ('wp_then:WP 'a) ('wp_else:WP 'a) ('post:Post 'a) = 
-                 (if 'p 
-                  then 'wp_then 'post
-                  else 'wp_else 'post)
-             type ite_wlp ('a:Type) ('wlp_cases:WP 'a) ('post:Post 'a) =
-                 (forall (a:'a). 'wlp_cases (fun a' -> a=!=a') \/ 'post a)
-             type ite_wp ('a:Type) ('wlp_cases:WP 'a) ('wp_cases:WP 'a) ('post:Post 'a) =
-                 (forall (a:'a). 'wlp_cases (fun a' -> a=!=a') \/ 'post a)
-                 /\ ('wp_cases (fun a -> True))
-             type wp_binop ('a:Type) ('wp1:WP 'a) ('op:Type -> Type -> Type) ('wp2:WP 'a) ('p:Post 'a) =
-                 'op ('wp1 'p) ('wp2 'p)
-             type wp_as_type ('a:Type) ('wp:WP 'a) = (forall ('p:Post 'a). 'wp 'p)
-             type close_wp ('a:Type) ('b:Type) ('wp:'b -> WP 'a) ('p:Post 'a) = (forall (b:'b). 'wp b 'p)
-             type close_wp_t ('a:Type) ('wp:Type -> WP 'a) ('p:Post 'a) = (forall ('b:Type). 'wp 'b 'p)
-             type assert_p ('a:Type) ('P:Type) ('wp:WP 'a) ('p:Post 'a) = ('P /\ 'wp 'p)
-             type assume_p ('a:Type) ('P:Type) ('wp:WP 'a) ('p:Post 'a) = ('P ==> 'wp 'p)
-             type null_wp ('a:Type) ('p:Post 'a) = (forall (x:'a). 'p x)
-             type trivial ('a:Type) ('wp:WP 'a) = 'wp (fun x -> True)
-             with Pure ('a:Type) ('pre:Pre) ('post:Post 'a) =
-                 PURE 'a
-                   (fun ('p:Post 'a) -> 'pre /\ (forall a. 'post a ==> 'p a)) (* WP *)
-                   (fun ('p:Post 'a) -> forall a. 'pre /\ 'post a ==> 'p a)   (* WLP *)
-             and Fact ('res:Type) ('p:Type) = Pure 'res True (fun r -> 'p)
-             (* and PURE ('a:Type) ('wp:WP 'a) ('wlp:WP 'a) =  *)
-             (*     Pure 'a ('wp (fun a -> True)) (fun a -> 'wlp (fun a' -> a==a')) *)
-             and Tot ('a:Type) =
-                 PURE 'a (fun 'p -> (forall (x:'a). 'p x)) (fun 'p -> (forall (x:'a). 'p x))
+             kind Post (a:Type) = a -> Type
+             kind WP (a:Type) = Post a -> Pre
+             type return (a:Type) (x:a) (p:Post a) = p x
+             type bind_wp  (a:Type) (b:Type) (wp1:WP a) (wlp1:WP a) 
+                                              (wp2: (a -> WP b)) (wlp2: (a -> WP b))
+                                               (p:Post b) = wp1 (fun a -> wp2 a p)
+             type bind_wlp (a:Type) (b:Type) (wlp1:WP a) 
+                                             (wlp2:(a -> WP b))
+                                             (p:Post b) = wlp1 (fun a -> wlp2 a p)
+             type if_then_else (a:Type) (p:Type) (wp_then:WP a) (wp_else:WP a) (post:Post a) = 
+                 (if p 
+                  then wp_then post
+                  else wp_else post)
+             type ite_wlp (a:Type) (wlp_cases:WP a) (post:Post a) =
+                 (forall (a:a). wlp_cases (fun a' -> a=!=a') \/ post a)
+             type ite_wp (a:Type) (wlp_cases:WP a) (wp_cases:WP a) (post:Post a) =
+                 (forall (a:a). wlp_cases (fun a' -> a=!=a') \/ post a)
+                 /\ (wp_cases (fun a -> True))
+             type wp_binop (a:Type) (wp1:WP a) (op:(Type -> Type -> Type)) (wp2:WP a) (p:Post a) =
+                 op (wp1 p) (wp2 p)
+             type wp_as_type (a:Type) (wp:WP a) = (forall (p:Post a). wp p)
+             type close_wp (a:Type) (b:Type) (wp:(b -> WP a)) (p:Post a) = (forall (b:b). wp b p)
+             type close_wp_t (a:Type) (wp:(Type -> WP a)) (p:Post a) = (forall (b:Type). wp b p)
+             type assert_p (a:Type) (q:Type) (wp:WP a) (p:Post a) = (q /\ wp p)
+             type assume_p (a:Type) (q:Type) (wp:WP a) (p:Post a) = (q ==> wp p)
+             type null_wp (a:Type) (p:Post a) = (forall (x:a). p x)
+             type trivial (a:Type) (wp:WP a) = wp (fun x -> True)
+             with Pure (a:Type) (pre:Pre) (post:Post a) =
+                 PURE a
+                   (fun (p:Post a) -> pre /\ (forall a. post a ==> p a)) (* WP *)
+                   (fun (p:Post a) -> forall a. pre /\ post a ==> p a)   (* WLP *)
+             and Fact (res:Type) (p:Type) = Pure res True (fun r -> p)
+             (* and PURE (a:Type) (wp:WP a) (wlp:WP a) =  *)
+             (*     Pure a (wp (fun a -> True)) (fun a -> wlp (fun a' -> a==a')) *)
+             and Tot (a:Type) =
+                 PURE a (fun (p:Post a) -> (forall (x:a). p x)) (fun (p:Post a) -> (forall (x:a). p x))
 }
 open Prims.PURE
-assume type bool
+
 assume type unit
 assume type int
 assume type char
@@ -95,11 +97,12 @@ assume type exn
 assume type HashMultiMap : Type -> Type -> Type
 type double = float
 type int32 = int
-logic type b2t (b:bool) = b==true
 
-type option 'a =
-  | None : option 'a
-  | Some : v:'a -> option 'a
+
+
+type option (a:Type) =
+  | None : option a
+  | Some : v:a -> option a
 
 assume type heap
 assume logic val SelHeap : #'a:Type -> heap -> ref 'a -> Tot 'a
